messageInvariantPrototypes/paxos/centralized/applicationProof.dfy
@@ -7,46 +7,6 @@ import opened UtilitiesLibrary
 import opened System
 import opened Obligations
 
-
-ghost predicate OneValuePerBallot(c: Constants, v: Variables)
-  requires v.WF(c)
-{
-  && OneValuePerBallotAcceptors(c, v)
-  && OneValuePerBallotLearners(c, v)
-  && OneValuePerBallotLeaderAndLearners(c, v)
-  && OneValuePerBallotLeaderAndAcceptors(c, v)
-}
-
-// Acceptors only have one value for each ballot
-ghost predicate OneValuePerBallotAcceptors(c: Constants, v: Variables)
-  requires v.WF(c)
-{
-  forall a1, a2 |
-    && c.ValidAcceptorIdx(a1)
-    && c.ValidAcceptorIdx(a2)
-    && v.acceptors[a1].acceptedVB.MVBSome?
-    && v.acceptors[a2].acceptedVB.MVBSome?
-    && v.acceptors[a1].acceptedVB.value.b 
-        == v.acceptors[a2].acceptedVB.value.b 
-  ::
-    v.acceptors[a1].acceptedVB.value.v
-        == v.acceptors[a2].acceptedVB.value.v
-}
-
-// Learners only have one value for each ballot
-ghost predicate OneValuePerBallotLearners(c: Constants, v: Variables)
-  requires v.WF(c)
-{
-  forall l1, l2, vb1, vb2 |
-    && c.ValidLearnerIdx(l1)
-    && c.ValidLearnerIdx(l2)
-    && vb1 in v.learners[l1].receivedAccepts.m
-    && vb2 in v.learners[l2].receivedAccepts.m
-    && vb1.b == vb2.b
-  ::
-    vb1.v == vb2.v
-}
-
 // Leaders and Learners only have one value for each ballot
 ghost predicate OneValuePerBallotLeaderAndLearners(c: Constants, v: Variables)
   requires v.WF(c)
@@ -55,18 +15,6 @@ ghost predicate OneValuePerBallotLeaderAndLearners(c: Constants, v: Variables)
     && c.ValidLeaderIdx(ldr)
     && c.ValidLearnerIdx(lnr)
     && VB(acceptedVal, ldr) in v.learners[lnr].receivedAccepts.m
-  ::
-    acceptedVal == v.leaders[ldr].Value()
-}
-
-// Leaders and Acceptors only have one value for each ballot
-ghost predicate OneValuePerBallotLeaderAndAcceptors(c: Constants, v: Variables)
-  requires v.WF(c)
-{
-  forall ldr, acc, acceptedVal |
-    && c.ValidLeaderIdx(ldr)
-    && c.ValidAcceptorIdx(acc)
-    && v.acceptors[acc].HasAccepted(VB(acceptedVal, ldr))
   ::
     acceptedVal == v.leaders[ldr].Value()
 }
@@ -83,24 +31,13 @@ ghost predicate LearnerValidReceivedAccepts(c: Constants, v: Variables)
     c.ValidAcceptorIdx(e)
 }
 
-// Learner's receivedAccepts contain valid leader ballots
-ghost predicate LearnerValidReceivedAcceptsKeys(c: Constants, v: Variables)
-  requires v.WF(c)
-{
-  forall lnr:LearnerId, vb:ValBal |
-    && c.ValidLearnerIdx(lnr)
-    && vb in v.learners[lnr].receivedAccepts.m
-  ::
-    c.ValidLeaderIdx(vb.b)
-}
-
 ghost predicate LearnerReceivedAcceptImpliesProposed(c: Constants, v: Variables) 
   requires v.WF(c)
-  requires LearnerValidReceivedAcceptsKeys(c, v)
 {
   forall lnr:LearnerId, vb:ValBal |
     && c.ValidLearnerIdx(lnr)
     && vb in v.learners[lnr].receivedAccepts.m
+    && c.ValidLeaderIdx(vb.b)
   ::
     && v.LeaderCanPropose(c, vb.b)
     && v.leaders[vb.b].Value() == vb.v
@@ -270,7 +207,6 @@ ghost predicate ApplicationInv(c: Constants, v: Variables)
   requires v.WF(c)
 {
   && LearnerValidReceivedAccepts(c, v)
-  && LearnerValidReceivedAcceptsKeys(c, v)
   && LearnedImpliesQuorumOfAccepts(c, v)
   && LearnerReceivedAcceptImpliesProposed(c, v)
   && LearnerReceivedAcceptImpliesAccepted(c, v)
@@ -314,8 +250,8 @@ lemma InvInductive(c: Constants, v: Variables, v': Variables)
   requires Next(c, v, v')
   ensures Inv(c, v')
 {
+  assert OneValuePerBallotLeaderAndLearners(c, v);
   InvNextLearnerValidReceivedAccepts(c, v, v');
-  InvNextLearnerValidReceivedAcceptsKeys(c, v, v');
   InvNextLearnerReceivedAcceptImpliesProposed(c, v, v');
   InvNextAcceptorValidPromisedAndAccepted(c, v, v');
   InvNextAcceptorAcceptedImpliesProposed(c, v, v');
@@ -344,12 +280,6 @@ lemma InvNextLearnerValidReceivedAccepts(c: Constants, v: Variables, v': Variabl
   requires Inv(c, v)
   requires Next(c, v, v')
   ensures LearnerValidReceivedAccepts(c, v')
-{}
-
-lemma InvNextLearnerValidReceivedAcceptsKeys(c: Constants, v: Variables, v': Variables)
-  requires Inv(c, v)
-  requires Next(c, v, v')
-  ensures LearnerValidReceivedAcceptsKeys(c, v')
 {}
 
 lemma InvNextLearnerReceivedAcceptImpliesProposed(c: Constants, v: Variables, v': Variables)
@@ -586,7 +516,7 @@ lemma InvNextChosenValImpliesAcceptorOnlyAcceptsVal(c: Constants, v: Variables, 
   
   // prereqs for LeaderHearsDifferentValueFromChosenImpliesFalse
   requires AcceptorAcceptedImpliesProposed(c, v')
-  requires OneValuePerBallot(c, v')
+  requires OneValuePerBallotLeaderAndLearners(c, v')
   requires LeaderHighestHeardUpperBound(c, v')
   requires LeaderHearedImpliesProposed(c, v')
   requires ChosenImpliesProposingLeaderHearsChosenBallot(c, v')
@@ -617,7 +547,7 @@ lemma InvNextChosenValImpliesAcceptorOnlyAcceptsVal(c: Constants, v: Variables, 
 lemma InvNextChosenValImpliesLeaderOnlyHearsVal(c: Constants, v: Variables, v': Variables)
   requires Inv(c, v)
   requires Next(c, v, v')
-  requires OneValuePerBallot(c, v')
+  requires OneValuePerBallotLeaderAndLearners(c, v')
   requires LeaderHighestHeardUpperBound(c, v')
   requires LeaderHearedImpliesProposed(c, v')
   requires ChosenImpliesProposingLeaderHearsChosenBallot(c, v')
@@ -653,7 +583,7 @@ lemma LeaderHearsDifferentValueFromChosenImpliesFalse(c: Constants, v: Variables
   requires v.leaders[ldr].highestHeardBallot.value >= chosen.b
   requires v.leaders[ldr].Value() != chosen.v
   requires chosen.b < ldr
-  requires OneValuePerBallot(c, v)
+  requires OneValuePerBallotLeaderAndLearners(c, v)
   requires LeaderHighestHeardUpperBound(c, v)
   requires LeaderHearedImpliesProposed(c, v)
   requires ChosenImpliesProposingLeaderHearsChosenBallot(c, v)
@@ -701,7 +631,10 @@ ghost predicate AtMostOneChosenVal(c: Constants, v: Variables)
   requires v.WF(c)
 {
   forall vb1, vb2 | Chosen(c, v, vb1) && Chosen(c, v, vb2) 
-  :: vb1.v == vb2.v
+  :: 
+    && c.ValidLeaderIdx(vb1.b)
+    && c.ValidLeaderIdx(vb2.b)
+    && vb1.v == vb2.v
 }
 
 
